src/Correctness/BooleanCorrectnessSkeleton.v
@@ -1,0 +1,121 @@
+Require Import Core.Core Core.StructNormalizer VstLib Callback.Dummy
+        Boolean.Exec ErrorWithWriter DWT.Vst.
+Require Import VST.floyd.proofauto.
+Require Import Clight.dummy Clight.BOOLEAN.
+Require Import Core.Notations. 
+Require Import Boolean.Exec AbstractSpec Lib Prim.Exec.
+Require Import Clight.dummy Clight.BOOLEAN.
+
+Hypothesis der_encoder_correctness : forall td b ls z,
+  decoder_type td = BOOLEAN_t ->
+  bool_encoder td b [] = inr (ls, z) ->
+  DER (BOOLEAN b) ls.
+
+Hypothesis ber_decoder_correctness : forall td ls b z,
+    decoder_type td = BOOLEAN_t ->
+    bool_decoder td ls = Some (b, z) ->
+    BER (BOOLEAN b) ls.
+
+Hypothesis boolean_roundtrip : forall td ls b z,
+    decoder_type td = BOOLEAN_t ->
+    bool_encoder td b [] = inr (ls, z) ->
+    bool_decoder td ls = Some (b, z).
+
+Definition bool_der_encode_spec : ident * funspec :=
+  DECLARE _BOOLEAN_encode_der
+    (* parameters *)
+    WITH res: val,  sptr_p : val, sptr_val : int, 
+         td_p : val, td : TYPE_descriptor,
+         tag_mode : Z, tag : Z,
+         app_key_p : val,
+         buf_b : block, buf_ofs : ptrofs, cb_p : val
+    (* PRECONDITION *)
+    PRE [tptr enc_rval_s, tptr type_descriptor_s, tptr tvoid, tint, 
+         tuint, tptr cb_type, tptr tvoid]
+      PROP (decoder_type td = BOOLEAN_t;
+            isptr (Vptr buf_b buf_ofs))
+      PARAMS (res; td_p; sptr_p; Vint (Int.repr tag_mode);
+              Vint (Int.repr tag); cb_p; app_key_p)
+      GLOBALS ()
+      SEP (data_at_ Tsh enc_rval_s res;
+           data_at_ Tsh type_descriptor_s td_p; 
+           data_at Tsh tint (Vint sptr_val) sptr_p;
+           data_at_ Tsh tvoid app_key_p;
+           valid_pointer cb_p)
+    (* POSTCONDITION *)
+    POST [tvoid]
+      PROP ()
+      LOCAL ()
+      let res_val := 
+          match evalErrW (bool_encoder td (bool_of_int sptr_val)) [] with 
+                     | Some v => mk_enc_rval v Vzero 
+                     | None => mk_enc_rval (-1) sptr_p end in
+      SEP (data_at Tsh enc_rval_s res_val res;
+           data_at_ Tsh type_descriptor_s td_p; 
+           data_at Tsh tint (Vint sptr_val) sptr_p;
+           data_at_ Tsh tvoid app_key_p;
+           valid_pointer cb_p).
+
+(* We are proving: forall x in parameters, 
+   the separation logic triple 
+   PRECONDITION {f_BOOLEAN_encode_der} POSTCONDITION
+   holds *)
+
+Hypothesis bool_der_encode :
+  semax_body Vprog Gprog (normalize_function f_BOOLEAN_encode_der composites)
+             bool_der_encode_spec.
+
+Definition bool_ber_decode_spec : ident * funspec :=
+  DECLARE _BOOLEAN_decode_ber
+    (* parameters *)
+    WITH ctx_p : val, ctx : val, td_p : val, td : TYPE_descriptor,
+         bv_pp : val, buf_p : val, buf : list byte,
+         res_p : val, size : Z, tag_mode : Z, bv_p : val
+    (* PRECONDITION *)
+    PRE [tptr asn_dec_rval_s, tptr asn_codec_ctx_s, tptr type_descriptor_s,
+          tptr (tptr tvoid), tptr tvoid, tuint, tint] 
+      PROP (is_pointer_or_null bv_p; decoder_type td = BOOLEAN_t; 
+            0 <= size <= Int.max_signed;
+            Zlength buf = size)
+      PARAMS (res_p; ctx_p; td_p; bv_pp; buf_p; Vint (Int.repr size);
+                Vint (Int.repr tag_mode))
+      GLOBALS ()
+      SEP (valid_pointer bv_p;
+           if eq_dec bv_p nullval 
+           then emp
+           else data_at_ Ews tint bv_p ; 
+           data_at Tsh asn_codec_ctx_s ctx ctx_p;
+           data_at_ Tsh type_descriptor_s td_p;
+           data_at Tsh (tarray tuchar (Zlength buf)) (map Vubyte buf) buf_p;
+           data_at Tsh (tptr tvoid) bv_p bv_pp;
+           data_at_ Tsh asn_dec_rval_s res_p)
+    (* POSTCONDITION *)
+    POST [tvoid] 
+      PROP ()
+      LOCAL ()
+      SEP (valid_pointer bv_p;
+           data_at Tsh asn_codec_ctx_s ctx ctx_p;
+           data_at_ Tsh type_descriptor_s td_p;
+           data_at Tsh (tarray tuchar (len buf)) (map Vubyte buf) buf_p;
+           let res_val := match bool_decoder td buf with
+                          | Some (r, c) => ((Vzero, Vint (Int.repr c)),
+                                           (Vubyte (byte_of_bool r)))
+                          | None => ((Vint (Int.repr 2), Vzero), Vone)
+                          end in
+           EX v : val,
+                  EX ls : list val, data_at Tsh (tptr tvoid) v bv_pp *
+                                    if eq_dec v nullval 
+                                    then data_at Tsh asn_dec_rval_s
+                                                 (Vint (Int.repr 2), Vzero) res_p
+                                    else data_at Tsh asn_dec_rval_s
+                                                 (fst res_val) res_p *
+                                         data_at Ews tint (snd res_val) v).
+                                    
+(* We are proving: forall x in parameters, 
+   the separation logic triple 
+   PRECONDITION {f_BOOLEAN_decode_ber} POSTCONDITION
+   holds *)
+
+Hypothesis bool_ber_decode_correctness : 
+  semax_body Vprog Gprog (normalize_function f_BOOLEAN_decode_ber composites) 
+             bool_ber_decode_spec.
