src/Correctness/IntegerCorrectness.v
@@ -1,0 +1,43 @@
+Require Import Int.Exec AbstractSpec Lib Prim.Exec.
+Require Import Core.Core Core.Notations Core.Tactics.
+From ExtLib.Structures Require Import Monad MonadWriter Monoid.
+From ExtLib.Data Require Import Monads.OptionMonad List.
+
+Import MonadNotation.
+
+Open Scope monad.
+
+(* Exec spec *)
+(*
+Parameter int_to_byte : Z -> list byte.
+Parameter int_of_byte : list byte -> Z.
+
+Definition int_encoder : TYPE_descriptor -> Z -> errW1 asn_enc_rval :=
+  fun td i => int_encoder td (int_to_byte i). 
+
+Definition int_decoder : TYPE_descriptor -> list byte -> option (list byte * Z) :=
+  fun td ls => int_decoder td ls.
+
+(* Exec spec correctness wrt to the relational spec *)
+
+Parameter int_der_encoder_correctness : forall td i z ls ,
+    decoder_type td = INTEGER_t ->
+    int_encoder td i [] = inr (ls, z) ->
+    DER (INTEGER i) ls.
+
+Parameter int_ber_decoder_correctness : forall td ls ls' z,
+    decoder_type td = INTEGER_t ->
+    int_decoder td ls = Some (ls', z) ->
+    BER (INTEGER z) ls.
+
+(* Roundtrip *)
+
+Parameter int_roundtrip : forall td ls i z,
+    decoder_type td = INTEGER_t ->
+    int_encoder td i nil = inr (ls, encode z) ->
+    int_decoder td ls = Some ([], i).
+
+Require Import Primitive.Int.VstDec.
+
+(* Check int_der_encode_spec. *)
+*)
